* Redefined dfs with Iteration + Program Fixpoint
  The idea follows 15.3 of Coq'Art:
  1) first define a denotation-like computation, which is a bounded iteration, 
     returns bot when bound reaches.
  2) then we prove that their must exist a bound for a concrete
     functional, say DFS. So, we proved termination
  3) by ternimation proofs, we prove the fixpoint equation of DFS
  4) by the fixpoint equation, we can prove other DFS' properties by
     well-founded induction easily.

  This design follows the RecursiveDefinition contribution: 
     http://coq.inria.fr/pylons/contribs/view/RecursiveDefinition/v8.3
  The Coq extension is not sufficient to encode DFS. But the structure
  is very similar. (2) is proved by Program Fixpoint, rather than the 
  refine tactic.

  The benefits of the design are
  1) separate computation, termination, specification of a function
     completely. So, we do not need to reason about the dependent programming 
     in Coq, which is very ad-hoc for different functions.

     Although we use Program Fixpoint to use Termination, we never need
     to reason about that that proof.

  2) it does not introduce any runtime overhead. The existence of the
     bound of DFS is proved in the meta-level, and eliminated by Coq's
     extraction.
  3) the structure is very generic, and can be used to encode other 
     recursions in Vellvm.

  NOTE: In general, if a function can be defined w/o reasoning about 
    additional properties that can be changed in different recursions.
    Program Fixpoint is good. For example, "div n m" is fine, whose
    termination needs m>0, but this condition is same at each recursion.

    But, to show that DFS works on a well-founded relation (lex-order),
    we must know that all visited nodes are in CFG (therefore, it is a 
    infinte chain), which is a property that changes at each call.   
    Such a highly dependent definition is hard to reason about. 

    One solution is that we can prove all properties of DFS when
    defining DFS, namely making the specification of DFS stronger. We
    may try this alternative if neccessary.

* We proved the DFS post-order property in r3996 of the new DFS. The
  proof is by wf-induction and using fix-equation at each recursion,
  otherwise, looks very common.

* The performance of the new DFS is same to the old one. The extracted
  code are the same. Because the termination proof is the definition of 
  the new DFS, which is exactly the definition of the old DFS.

* exported tactics from CPDT.



git-svn-id: https://webdav.seas.upenn.edu/svn/sol/vol@3997 eef5ea85-cc2e-0410-bd84-0fae1f012da8

src3.0/Vellvm/Dominators/dfs.v
@@ -90,14 +90,14 @@ Proof.
   omega.
 Qed.
 
-Definition stk_takes_succs succs (stk : list Frame) : Prop :=
+Definition stk_in_children succs (stk : list Frame) : Prop :=
 List.Forall (fun fr : Frame => 
              incl (Fr_scs fr) (XATree.children_of_tree succs)) stk.
 
-Hint Unfold stk_takes_succs.
+Hint Unfold stk_in_children.
 
 Lemma find_next_visit_in_stk_spec1: forall succs visited (stk : list Frame)
-  (Hp : stk_takes_succs succs stk)  
+  (Hp : stk_in_children succs stk)  
   po (next : l) (stk' : list Frame) po'
   (Hfind : inl (next, stk', po') = find_next_visit_in_stk succs visited po stk),
   Forall 
@@ -142,7 +142,7 @@ Qed.
 Lemma find_next_visit_in_stk_spec3: forall succs visited 
   (Hinc: incl (XATree.parents_of_tree visited) (XATree.children_of_tree succs))
   (stk : list Frame) 
-  (Hp : stk_takes_succs succs stk)
+  (Hp : stk_in_children succs stk)
   (next : l) (stk' : list Frame) po po'
   (Hfind : inl (next, stk', po') =
                    find_next_visit_in_stk succs visited po stk),
@@ -172,7 +172,7 @@ Lemma find_next_visit_in_stk_spec2: forall (succs : ATree.t ls)
   (visited : ATree.t unit)
   (Hinc : incl (XATree.parents_of_tree visited) (XATree.children_of_tree succs))
   (stk : list Frame)
-  (Hp : stk_takes_succs succs stk)
+  (Hp : stk_in_children succs stk)
   (next : l) (stk' : list Frame) po po'
   (Hfind : inl (next, stk', po') = find_next_visit_in_stk succs visited po stk),
   incl (XATree.parents_of_tree (ATree.set next tt visited))
@@ -199,9 +199,9 @@ Proof.
         apply List.in_map with (f:=fst) in H2; auto.
 Qed.
 
-Program Fixpoint dfs_aux (succs: ATree.t ls)
+Program Fixpoint dfs_aux1 (succs: ATree.t ls)
   (visited: ATree.t unit) (po:PostOrder) (stk: list Frame) 
-  (Hp: stk_takes_succs succs stk /\
+  (Hp: stk_in_children succs stk /\
        incl (XATree.parents_of_tree visited) (XATree.children_of_tree succs))
   {measure 
      (length (XATree.children_of_tree succs) - 
@@ -209,7 +209,7 @@ Program Fixpoint dfs_aux (succs: ATree.t ls)
   : PostOrder :=
   match find_next_visit_in_stk succs visited po stk with
   | inr po' => po'
-  | inl (next, stk', po') => dfs_aux succs (ATree.set next tt visited) po' stk' _
+  | inl (next, stk', po') => dfs_aux1 succs (ATree.set next tt visited) po' stk' _
   end.
 Next Obligation.
   split.
@@ -220,6 +220,105 @@ Next Obligation.
   eapply find_next_visit_in_stk_spec3; eauto.
 Qed.
 
+(************************)
+
+Fixpoint iter (A:Type) (n:nat) (F:A->A)(g:A) : A :=
+  match n with
+  | O => g
+  | S p => F (iter A p F g)
+  end.
+
+Definition dfs_aux_type : Type :=
+  forall (succs: ATree.t ls)
+  (visited: ATree.t unit) (po:PostOrder) (stk: list Frame),
+  PostOrder.
+
+Definition dfs_aux_F (f: dfs_aux_type)
+  (succs: ATree.t ls)
+  (visited: ATree.t unit) (po:PostOrder) (stk: list Frame) 
+  : PostOrder :=
+  match find_next_visit_in_stk succs visited po stk with
+  | inr po' => po'
+  | inl (next, stk', po') => f succs (ATree.set next tt visited) po' stk'
+  end.
+
+Require Import cpdt_tactics.
+
+Lemma find_next_visit_in_stk_spec12: forall (succs : ATree.t ls) 
+  (visited : ATree.t unit) (po : PostOrder) (stk : list Frame)
+  (H : stk_in_children succs stk /\
+       incl (XATree.parents_of_tree visited) (XATree.children_of_tree succs))
+  next stk' po'
+  (Heq_anonymous : inl (next, stk', po') =
+                   find_next_visit_in_stk succs visited po stk),
+  stk_in_children succs stk' /\
+  incl (XATree.parents_of_tree (ATree.set next tt visited))
+       (XATree.children_of_tree succs).
+Proof.
+  intros.
+  destruct_conjs.
+  split.
+    eapply find_next_visit_in_stk_spec1; eauto.
+    eapply find_next_visit_in_stk_spec2; eauto.
+Qed.
+
+Program Fixpoint dfs_aux_terminates (succs: ATree.t ls)
+  (visited: ATree.t unit) (po:PostOrder) (stk: list Frame) 
+  (Hp: stk_in_children succs stk /\
+       incl (XATree.parents_of_tree visited) (XATree.children_of_tree succs))
+  {measure 
+     (length (XATree.children_of_tree succs) - 
+      length (XATree.parents_of_tree visited))%nat }
+  : { po':PostOrder | 
+      exists p:nat, 
+        forall k, (p < k)%nat ->
+        forall g:dfs_aux_type,
+          iter _ k dfs_aux_F g succs visited po stk = po' } :=
+  match find_next_visit_in_stk succs visited po stk with
+  | inr po' => po'
+  | inl (next, stk', po') => 
+      let _:=dfs_aux_terminates succs (ATree.set next tt visited) po' stk' _ in
+      _
+  end.
+Next Obligation.
+  exists O; intros k; case k.
+    intros. crush.
+
+    intros k' Hltp g; simpl; unfold dfs_aux_F at 1.
+    rewrite <- Heq_anonymous; auto.
+Qed.
+Next Obligation.
+  eapply find_next_visit_in_stk_spec12; eauto.
+Qed.
+Next Obligation.
+  eapply find_next_visit_in_stk_spec3; eauto.
+Qed.
+Next Obligation.
+  case dfs_aux_terminates with (succs0:=succs)
+    (visited0:=ATree.set next tt visited)(po:=po')(stk:=stk'); auto with arith.
+    eapply find_next_visit_in_stk_spec12; eauto.
+    eapply find_next_visit_in_stk_spec3; eauto.
+
+  intros x; intros Hex.
+  exists x.
+  elim Hex; intros p Heq.
+  exists (S p).
+  intros k.
+  case k.
+    intros. crush.
+  
+    intros k' Hplt g; simpl.
+    unfold dfs_aux_F at 1.
+    rewrite <- Heq_anonymous; auto with arith.
+Qed.
+
+Definition dfs_aux (succs: ATree.t ls)
+  (visited: ATree.t unit) (po:PostOrder) (stk: list Frame) 
+  (Hp: stk_in_children succs stk /\
+       incl (XATree.parents_of_tree visited) (XATree.children_of_tree succs))
+  : PostOrder :=
+  let (po', _) := dfs_aux_terminates succs visited po stk Hp in po'.
+
 Program Definition dfs (succs: ATree.t ls) (entry:l) (pinit:positive) : PostOrder :=
 dfs_aux succs (ATree.empty unit) (mkPO pinit (ATree.empty positive)) 
   (mkFrame entry (succs!!!entry)::nil) _.
@@ -229,6 +328,45 @@ Next Obligation.
       apply XATree.children_in_children_of_tree.
     rewrite XATree.parents_of_empty_tree. 
     intros x Hin. tauto.
+Qed.
+
+Require Import Max.
+
+Lemma dfs_aux_fix_eqn: forall succs visited po stk Hp po1
+  (Heq: dfs_aux succs visited po stk Hp = po1),
+  match find_next_visit_in_stk succs visited po stk with
+  | inr po' => po' = po1
+  | inl (next, stk', po') => 
+      exists Hp', dfs_aux succs (ATree.set next tt visited) po' stk' Hp' = po1
+  end.
+Proof.
+  unfold dfs_aux.
+  intros until po1.
+  case (dfs_aux_terminates succs visited po stk Hp).
+  intros v Hex1 EQ. subst.
+  elim Hex1.
+  intros p Heq1.
+  caseEq (find_next_visit_in_stk succs visited po stk).
+    intros [[next stk'] po'] Hfind.
+    eapply find_next_visit_in_stk_spec12 in Hp; eauto.
+    exists Hp.
+    case (dfs_aux_terminates succs (ATree.set next tt visited) po' stk' Hp).    
+    intros v' Hex2.
+    elim Hex2. 
+    intros p' Heq2.
+    rewrite <- Heq1 with (k:=S (S (max p p')))
+                         (g:=fun _ _ _ _  =>po).
+    rewrite <- Heq2 with (k:=S (max p p'))
+                         (g:=fun _ _ _ _ =>po).
+      simpl. unfold dfs_aux_F at 3. rewrite Hfind. auto.
+      eauto using le_max_l with arith.
+      eauto using le_max_r with arith.
+
+    intros po0 Hfind.
+    rewrite <- Heq1 with (k:=S p)
+                         (g:=fun _ _ _ _  =>po).
+      simpl. unfold dfs_aux_F at 1. rewrite Hfind. auto.
+      eauto using le_max_l with arith.
 Qed.
 
 Fixpoint stk_isa_path (succs: ATree.t ls) (entry:atom) (stk:list Frame) : Prop :=
@@ -252,6 +390,10 @@ Definition wf_aorder_aux (succs: ATree.t ls) (entry:atom) (po:PostOrder)
       ((exists p2, (PO_a2p po) ! a2 = Some p2 /\ (p2 > p1)%positive) \/
        node_in_stk a2 stk).
 
+Definition stk_takes_succs succs (stk : list Frame) : Prop :=
+List.Forall (fun fr : Frame => 
+             incl (Fr_scs fr) (succs !!! (Fr_name fr))) stk.
+
 Definition wf_stack (succs: ATree.t ls) (entry:atom) (po:PostOrder) 
   (stk: list Frame) : Prop :=
 stk_isa_path succs entry stk /\
@@ -269,18 +411,342 @@ Definition dfs_aux_wf_stack_prop (n:nat) : Prop := forall (succs: ATree.t ls)
   (Heq: n = (length (XATree.children_of_tree succs) - 
              length (XATree.parents_of_tree visited))%nat)
   entry (po1:PostOrder) (stk: list Frame) 
-  (Hp: stk_takes_succs succs stk /\
+  (Hp: stk_in_children succs stk /\
        incl (XATree.parents_of_tree visited) (XATree.children_of_tree succs))
-  po2 (Hdsf: dfs_aux succs visited po1 stk Hp = po2)
+  po2 (Hdfs: dfs_aux succs visited po1 stk Hp = po2)
   (Hwf: wf_stack succs entry po1 stk),
   wf_aorder succs entry (PO_a2p po2).
 
+Ltac fill_holes_in_ctx := (* from push_iter.v *)
+let fill e H :=
+  match goal with
+  | H1: _ = e |- _ => rewrite <- H1 in H
+  | H1: e = _ |- _ => rewrite H1 in H
+  end
+in
+repeat match goal with
+| H: match ?e with
+     | Some _ => _
+     | None => _
+     end |- _ => fill e H
+| H: match ?e with
+     | inl _ => _
+     | inr _ => _
+     end |- _ => fill e H
+end.
+
+Lemma find_next_visit_in_stk_inl_spec: forall succs visited po stk re
+  (Heq: find_next_visit_in_stk succs visited po stk = inl re),
+  stk <> nil.
+Proof.
+  induction stk as [|[v scs] stk]; simpl; intros; congruence.
+Qed.
+
+Lemma find_next_visit_in_stk__stk_isa_path: forall succs entry 
+  stk (Hwfstk: stk_takes_succs succs stk) visited
+  po (Hwf: stk_isa_path succs entry stk) next stk' po'
+  (Heq: find_next_visit_in_stk succs visited po stk = inl (next, stk', po')),
+  stk_isa_path succs entry stk'.
+Proof.
+  induction 1 as [|[v scs] stk IH]; simpl; intros.
+    congruence.
+
+    inv_mbind_app.
+      destruct_let.
+      uniq_result.
+      split; auto.
+        apply find_next_visit_in_scs_spec in HeqR.
+        destruct_conjs.
+        apply IH. apply H. auto with coqlib.
+        
+      apply IHHwfstk in Heq; auto.
+      apply find_next_visit_in_stk_inl_spec in Heq. 
+      destruct stk as [|[]]; try congruence. 
+        tauto.
+Qed.
+
+Lemma find_next_visit_in_stk__stk_takes_succs: forall succs stk visited
+  (Hwf: stk_takes_succs succs stk) po next stk' po'
+  (Heq: find_next_visit_in_stk succs visited po stk = inl (next, stk', po')),
+  stk_takes_succs succs stk'.
+Proof.
+  induction 1 as [|[v scs] stk IH]; simpl; intros.
+    congruence.
+
+    inv_mbind_app; eauto 2.
+      destruct_let.
+      uniq_result.
+      constructor.
+        simpl. intro x; auto.
+        constructor; auto.
+          simpl. intro x; intros Hin. apply IH. simpl.
+          apply find_next_visit_in_scs_spec in HeqR.
+          destruct_conjs. apply H. auto with coqlib.
+Qed.
+
+Lemma node_in_stk_push: forall a2 hd v scs l1 stk
+  (Hnd: node_in_stk a2 ({| Fr_name := v; Fr_scs := scs |} :: stk)),
+  node_in_stk a2 (hd :: {| Fr_name := v; Fr_scs := l1 |} :: stk).
+Proof.
+  intros.
+  destruct Hnd as [stk1 [stk2 [scs' Hin]]].
+  destruct stk1 as [|fr1 stk1].
+    inv Hin.
+    exists [hd]. exists stk2. exists l1. simpl_env. auto.
+
+    inv Hin.
+    exists (hd::{|Fr_name:=v; Fr_scs:=l1|}::stk1). 
+    exists stk2. exists scs'. simpl_env. auto.
+Qed.
+
+Lemma push_wf_aorder_aux: forall (entry : atom) (succs : ATree.t ls)
+  (v : l) (scs : ls) (stk : list Frame) (next : l) (po' : PostOrder) (l1 : ls)
+  (Hwf : wf_aorder_aux succs entry po'
+           ({| Fr_name := v; Fr_scs := scs |} :: stk)),
+  wf_aorder_aux succs entry po'
+    ({| Fr_name := next; Fr_scs := succs !!! next |}
+     :: {| Fr_name := v; Fr_scs := l1 |} :: stk).
+Proof.
+  intros.
+  intros a1 p1 Hget1.
+  apply Hwf in Hget1.
+  destruct Hget1 as [J1 J2].
+  split; auto.
+    intro J3.
+    apply J2 in J3.
+    destruct J3 as [a2 [J3 J4]].
+    exists a2.
+    split; auto.
+      destruct J4 as [J4 | J4]; auto.
+        right. eapply node_in_stk_push; eauto.
+Qed.
+
+Lemma Plt_succ: forall (x: positive), (x < (Psucc x))%positive.
+Proof. apply Pcompare_p_Sp. Qed.
+
+Hint Resolve Plt_lt_succ Plt_succ: positive.
+
+Lemma node_in_stk_hd: forall Fr_name0 Fr_scs0 stk,
+  node_in_stk Fr_name0 ({| Fr_name := Fr_name0; Fr_scs := Fr_scs0 |} :: stk).
+Proof.
+  exists nil. exists stk. exists Fr_scs0. auto.
+Qed.
+
+Lemma node_in_stk_pop: forall a2 v scs fr stk
+  (Hin: node_in_stk a2
+           ({| Fr_name := v; Fr_scs := scs |}
+            :: fr :: stk))
+  (Hneq: a2 <> v),
+  node_in_stk a2 (fr :: stk).
+Proof.
+  intros.
+  destruct Hin as [stk1 [stk2 [scs' Hin]]].
+  destruct stk1 as [|fr1 stk1].
+    inv Hin. congruence.
+
+    inv Hin.
+    rewrite H1. unfold node_in_stk. eauto.
+Qed.
+
+Lemma pop_wf_aorder_aux: forall (entry : atom) (succs : ATree.t ls)
+  (v : l) (scs : ls) (Fr_name0 : l) (Fr_scs0 : ls) (stk : list Frame)
+  (po : PostOrder) (Hin: In v succs !!! Fr_name0)
+  (Hwf0 : wf_aorder_aux succs entry po
+           ({| Fr_name := v; Fr_scs := scs |}
+            :: {| Fr_name := Fr_name0; Fr_scs := Fr_scs0 |} :: stk)),
+  wf_aorder_aux succs entry (postorder_inc po v)
+    ({| Fr_name := Fr_name0; Fr_scs := Fr_scs0 |} :: stk).
+Proof.
+  intros.
+  intros a1 p1 Hget.
+  destruct po as [cnt a2p].
+  simpl in Hget.
+  rewrite ATree.gsspec in Hget.
+  destruct_if.
+    simpl.
+    split.
+      auto with positive.
+
+      intros.
+      exists Fr_name0.
+      split.
+        apply XATree.make_predecessors_correct; auto.
+        right. apply node_in_stk_hd.
+
+     apply Hwf0 in H0.
+     simpl in H0.
+     destruct H0 as [J1 J2].
+     split.
+       simpl. auto with positive.
+      
+       intro J.
+       apply J2 in J.
+       destruct J as [a2 [J3 J4]].
+       destruct (eq_atom_dec a2 v); subst.
+         exists v.
+         split; auto.
+           left. 
+           exists cnt.
+             simpl.
+             rewrite ATree.gss.
+             split; auto.
+               apply ZC2. auto.
+
+         exists a2.
+         split; auto.
+           simpl.
+           destruct J4 as [[p2 [J4 J5]] | J4].
+             left. exists p2.
+             split; auto.
+               rewrite ATree.gso; auto.
+
+            right. eapply node_in_stk_pop; eauto.
+Qed.
+
+Lemma find_next_visit_in_stk__wf_aorder_aux: forall entry succs stk visited
+  (Hwf: stk_isa_path succs entry stk)
+  po (Hwf: wf_aorder_aux succs entry po stk) next stk' po'
+  (Heq: find_next_visit_in_stk succs visited po stk = inl (next, stk', po')),
+  wf_aorder_aux succs entry po' stk'.
+Proof.
+  induction stk as [|[v scs] stk]; simpl; intros.
+    congruence.
+
+    inv_mbind_app.
+      destruct_let.
+      uniq_result.
+      eapply push_wf_aorder_aux; eauto.
+
+      assert (Hneq:=Heq).
+      apply find_next_visit_in_stk_inl_spec in Hneq. 
+      destruct stk as [|[]]; try congruence. 
+      apply IHstk in Heq; try solve [auto | tauto].
+      eapply pop_wf_aorder_aux; try solve [eauto | tauto].
+Qed.
+
+Lemma find_next_visit_in_stk__wf_stack: forall entry succs stk visited
+  po (Hwf: wf_stack succs entry po stk) next stk' po'
+  (Heq: find_next_visit_in_stk succs visited po stk = inl (next, stk', po')),
+  wf_stack succs entry po' stk'.
+Proof.
+  intros.
+  destruct Hwf as [J1 [J2 J3]]. 
+  unfold wf_stack.
+  eapply find_next_visit_in_stk__wf_aorder_aux in J3; eauto.
+  eapply find_next_visit_in_stk__stk_isa_path in J1; eauto.
+  eapply find_next_visit_in_stk__stk_takes_succs in J2; eauto.
+Qed.
+
+Lemma node_notin_empty_stk: forall a2 (H:node_in_stk a2 nil), False.
+Proof.
+  unfold node_in_stk.
+  intros.
+  destruct_conjs.
+  symmetry in H2.
+  contradict H2.
+  apply app_cons_not_nil.
+Qed.
+
+Lemma node_in_single_stk: forall a2 entry scs
+  (Hnd: node_in_stk a2 ({| Fr_name := entry; Fr_scs := scs |} :: nil)),
+  a2 = entry.
+Proof.
+  unfold node_in_stk.
+  intros.
+  destruct_conjs.
+  destruct Hnd; inv H1; auto.
+    symmetry in H4.
+    contradict H4.
+    apply app_cons_not_nil.
+Qed.
+
+Lemma wf_aorder_aux__find_next_visit_in_stk_inr__wf_aorder: forall 
+  succs entry stk po1 (Hwf': stk_isa_path succs entry stk)
+  (Hwf : wf_aorder_aux succs entry po1 stk) po2 visited
+  (Heq: find_next_visit_in_stk succs visited po1 stk = inr po2),
+  wf_aorder succs entry (PO_a2p po2).
+Proof.
+  induction stk as [|[v scs] stk]; simpl; intros.
+    uniq_result.
+    intros a1 Hneq p1 Hget1.
+    apply Hwf in Hget1; auto.
+    destruct Hget1 as [_ Hget1].
+    apply Hget1 in Hneq.
+    destruct Hneq as [a2 [J1 [[p2 [J2 J3]]|]]].
+      eauto.
+      apply node_notin_empty_stk in H. tauto.
+
+    inv_mbind_app.
+      destruct_let. congruence.
+      destruct stk as [|[] stk].
+        simpl in Heq. uniq_result.       
+        destruct po1. simpl.
+        intros a1 Hneq p1 Hget1.
+        rewrite ATree.gso in Hget1; auto.
+        apply Hwf in Hget1; auto.
+        simpl in Hget1.
+        destruct Hget1 as [G Hget1].
+        apply Hget1 in Hneq.
+        destruct Hneq as [a2 [J1 [[p2 [J2 J3]]|J2]]].
+          destruct (eq_atom_dec a2 entry); subst.      
+            exists entry. exists PO_cnt0.
+            rewrite ATree.gss.   
+            repeat (split; auto).
+              apply ZC2. auto.
+        
+            exists a2. exists p2.
+            split; auto.
+              rewrite ATree.gso; auto.
+            
+          apply node_in_single_stk in J2. subst.
+          exists entry. exists PO_cnt0.
+          rewrite ATree.gss.   
+          repeat (split; auto).
+            apply ZC2. auto.
+
+        apply IHstk in Heq; try solve [auto | tauto].
+        eapply pop_wf_aorder_aux; try solve [eauto | tauto].
+Qed.
+
+Lemma wf_stack__find_next_visit_in_stk_inr__wf_aorder: forall succs entry po1 stk
+  (Hwf : wf_stack succs entry po1 stk) po2 visited
+  (Heq: find_next_visit_in_stk succs visited po1 stk = inr po2),
+  wf_aorder succs entry (PO_a2p po2).
+Proof.
+  intros.
+  destruct Hwf as [J1 [J2 J3]].
+  eapply wf_aorder_aux__find_next_visit_in_stk_inr__wf_aorder; eauto.
+Qed.
+
 Lemma dfs_aux_wf_stack_aux: forall n, dfs_aux_wf_stack_prop n.
-Admitted.
+Proof.
+  intros.
+  elim n using (well_founded_induction lt_wf).
+  unfold dfs_aux_wf_stack_prop.
+  intros x IH. intros.
+  apply dfs_aux_fix_eqn in Hdfs.
+  caseEq (find_next_visit_in_stk succs visited po1 stk).
+    intros [[next stk'] po'] Hfind; fill_holes_in_ctx.
+    destruct Hdfs as [Hp' Hdfs].
+    eapply IH with (y:=
+      (length (XATree.children_of_tree succs) -
+       length (XATree.parents_of_tree (ATree.set next tt visited)))%nat) 
+      in Hdfs; eauto.
+      subst.  
+      symmetry in Hfind.
+      destruct_conjs.
+      eapply find_next_visit_in_stk_spec3 in Hfind; eauto. 
+
+      eapply find_next_visit_in_stk__wf_stack; eauto. 
+
+    intros p Hfind; fill_holes_in_ctx.
+    subst.
+    eapply wf_stack__find_next_visit_in_stk_inr__wf_aorder; eauto.
+Qed.
 
 Lemma dfs_aux_wf_stack: forall (succs: ATree.t ls) entry
   (visited: ATree.t unit) (po1:PostOrder) (stk: list Frame) 
-  (Hp: stk_takes_succs succs stk /\
+  (Hp: stk_in_children succs stk /\
        incl (XATree.parents_of_tree visited) (XATree.children_of_tree succs))
   po2 (Hdsf: dfs_aux succs visited po1 stk Hp = po2)
   (Hwf: wf_stack succs entry po1 stk),
@@ -300,8 +766,10 @@ Proof.
   unfold dfs. intros.
   apply dfs_aux_wf_stack with (entry:=entry) in Hdfs; auto.
   split. constructor; auto.
-  split. constructor; simpl; auto.
-          apply XATree.children_in_children_of_tree.
+  split. 
+    constructor; simpl; auto.
+      intro x. auto.
+
     intros a1 p1 Hget.   
     rewrite ATree.gempty in Hget. congruence.
 Qed.
@@ -317,95 +785,87 @@ Lemma asuccs_psuccs_pres_order: forall ascs pscs aentry pentry a2p
   wf_porder pscs pentry.
 Admitted.
  
-(*
-Program Fixpoint dfs_aux' (succs: ATree.t ls) (todo: ls) 
-  {measure (length (XATree.children_of_tree succs))%nat }
-  : unit :=
-  match todo with
-  | nil => tt
-  | next::todo' => 
-      match succs!!!next with
-      | sc::scc' => dfs_aux' (ATree.set next scc' succs) (sc::todo'++[next])
-      | nil => dfs_aux' succs todo'
-      end
+(************************)
+
+Definition div_it_F (f:nat -> nat -> nat * nat) (n m:nat) :=
+  match le_gt_dec m n with
+  | left _ => let '(q, r) := f (n-m)%nat m in (S q, r)
+  | right _ => (O, n)
+  end.
+
+Program Fixpoint div_it_terminates n m (Hlt: (O < m)%nat) {measure n}
+  : { v:nat * nat | 
+      exists p:nat, 
+        forall k, (p < k)%nat ->
+        forall g:nat->nat->nat*nat,
+          iter _ k div_it_F g n m = v } :=
+  match le_gt_dec m n with
+  | left _ => let _ := div_it_terminates (n-m)%nat m _ in _
+  | right _ => (O, n)
   end.
 Next Obligation.
-  admit.
+  omega.
 Qed.
 Next Obligation.
-  admit.
+  case div_it_terminates with (n0:=(n-m)%nat)(m:=m); auto with arith.
+  intros [q r]; intros Hex.
+  exists (S q, r).
+  elim Hex; intros p Heq.
+  exists (S p).
+  intros k.
+  case k.
+    intros. crush.
+  
+    intros k' Hplt g; simpl.
+    unfold div_it_F at 1.
+    rewrite <- Heq_anonymous; auto with arith.
+    rewrite Heq; crush.
 Qed.
 Next Obligation.
-  admit.
+  exists O; intros k; case k.
+    intros. crush.
+    intros k' Hltp g; simpl; unfold div_it_F at 1.
+    rewrite <- Heq_anonymous; auto.
 Qed.
 
-Definition dfs_aux_wf_stack_prop (n:nat) : Prop := forall (succs: ATree.t ls) 
-  (visited: ATree.t unit) 
-  (Hp: incl (XATree.parents_of_tree visited) (XATree.children_of_tree succs))
-  (Heq: n = (length (XATree.children_of_tree succs) - 
-             length (XATree.parents_of_tree visited))%nat)
-  todo
-  (Hdsf: dfs_aux' succs visited todo Hp = tt), True.
+Definition div_it (n m:nat) (H:(O<m)%nat) : nat*nat :=
+  let (v, _) := div_it_terminates n m H in v.
 
-Ltac unfold_dfs_aux' :=
-match goal with
-| |- appcontext [dfs_aux' ?arg] =>
-   unfold dfs_aux'; unfold dfs_aux'_func;
-   Program.Wf.WfExtensionality.unfold_sub dfs_aux' arg;
-   repeat Program.Wf.fold_sub dfs_aux'_func
-(*;
-   repeat fold_dfs_aux
-*)
-end.
-
-Require Import Program.Wf.
-
-Lemma dfs_aux_wf_stack_aux: forall n, dfs_aux_wf_stack_prop n.
+Lemma div_it_fix_eqn: forall n m (h: (O<m)%nat),
+  div_it n m h =
+  match le_gt_dec m n with
+  | left _ => let '(q, r) := div_it (n-m)%nat m h in (S q, r)
+  | right _ => (O, n)
+  end.
 Proof.
-  induction n.
-admit.
+  intros n m h.
+  unfold div_it.
+  case (div_it_terminates n m h).
+  intros v Hex1.
+  case (div_it_terminates (n-m) m h).
+  intros v' Hex2.
+  elim Hex2. elim Hex1.
+  intros p Heq1 p' Heq2.
+  rewrite <- Heq1 with (k:=S (S (max p p')))
+                       (g:=fun x y =>v).
+  rewrite <- Heq2 with (k:=S (max p p'))
+                       (g:=fun x y =>v).
+    reflexivity.
+    eauto using le_max_l with arith.
+    eauto using le_max_r with arith.
+Qed.
 
-    unfold dfs_aux_wf_stack_prop.
-    intros until todo.
-unfold_dfs_aux'.
-simpl.
+Lemma div_it_correct1: forall m n (h: (O<n)%nat),
+  m = (fst (div_it m n h) * n + snd (div_it m n h))%nat.
+Proof.
+  intros m.
+  elim m using (well_founded_induction lt_wf).
+  intros m' Hrec n h.
+  rewrite div_it_fix_eqn.
+  case (le_gt_dec n m'); intros H; trivial.
+  pattern m' at 1. rewrite (le_plus_minus n m'); auto.
+  pattern (m'-n)%nat at 1.
+  rewrite Hrec with (m'-n)%nat n h; auto with arith.
+  case (div_it (m' - n) n h)%nat; crush.
+Qed.
 
-destruct todo. auto.
-destruct (visited ! l0).
-destruct R.
-
-fold_sub dfs_aux'_func.
-
-match goal with
-| |- appcontext [dfs_aux' ?arg] =>
-   unfold dfs_aux'; unfold dfs_aux'_func;
-   Program.Wf.WfExtensionality.unfold_sub dfs_aux' arg
-(*;
-   repeat Program.Wf.fold_sub dfs_aux_func;
-   repeat fold_dfs_aux
-*)
-end.
-    simpl.
-
- match goal with
-  | |- appcontext C[Fix_sub _ _ _ _ _ ?arg] =>
-       let app := context C [dfs_aux'_func arg] in
-       change app
-  end.
-
-match goal with
-| |- context [dfs_aux_func (existT _ ?a (existT _ _ (existT _ ?b _)))] => 
-     fold (dfs_aux a)
-end.
-
-
-   unfold dfs_aux.
-   unfold dfs_aux_func.
-   WfExtensionality.unfold_sub dfs_aux arg.
-
-
-
-
-    unfold_dfs_aux.
-
-*)
